Documentation.

src/dafny/smart/intdiffalgo/IncAlgoV1.dfy
@@ -16,22 +16,21 @@ include "../trees/CompleteTrees.dfy"
 include "../synthattribute/ComputeRootPath.dfy"
 include "../synthattribute/GenericComputation.dfy"
 include "../helpers/Helpers.dfy"
-// include "../synthattribute/Siblings.dfy"
-// include "../MerkleTrees.dfy"
 include "../paths/NextPathInCompleteTreesLemmas.dfy"
 include "../paths/PathInCompleteTrees.dfy"
 include "../seqofbits/SeqOfBits.dfy"
 include "../helpers/SeqHelpers.dfy"
 include "../trees/Trees.dfy"
 
+/**
+ *  Provide an algorithm to compute root value and left siblings on next path concurrently.
+ */
 module IncAlgoV1 {
  
     import opened CompleteTrees
     import opened ComputeRootPath
     import opened GenericComputation
     import opened Helpers
-    // import opened Siblings
-    // import opened MerkleTrees
     import opened NextPathInCompleteTreesLemmas
     import opened PathInCompleteTrees
     import opened SeqOfBits
@@ -45,25 +44,21 @@ module IncAlgoV1 {
      *  @param  left        The values of the left siblings of nodes on path `p`.
      *  @param  right       The values of the left siblings of nodes on path `p`.
      *  @param  seed        The value at nodeAt(p).
-     *  @param  valOnPAt    The values of the nodes on the path p.
      *  @param  f           The binary operation to compute.
      *  @returns            The value of diff at the root and a vector of values of
      *                      for the left siblings on nextPath(p).
      */
     function computeRootAndLeftSiblingsUp<T>(
-        p : seq<bit>, left : seq<T>, right : seq<T>,  f : (T, T) -> T, seed: T, valOnPAt: seq<T>) : (T, seq<T>)
-        requires |p| == |left| == |right| == |valOnPAt|
+        p : seq<bit>, left : seq<T>, right : seq<T>,  f : (T, T) -> T, seed: T) : (T, seq<T>)
+        requires |p| == |left| == |right| 
         requires |p| >= 1
-        /*  This post-condition follows easily from the defs of the two functions.
-         *  The fact that computeRootAndLeftSiblingsUp.0 is the same as
-         *  computeRootPath requires some hints (ncluding this post-condition) 
-         *  and is proved in computeRootAnSiblingsIsCorrect.
-         */
-        ensures 
-            computeRootAndLeftSiblingsUp(p, left, right, f, seed, valOnPAt).1 
-            == 
-            computeLeftSiblingOnNextPath(p, valOnPAt, left)
         
+        ensures computeRootAndLeftSiblingsUp(p, left, right, f, seed).0 
+            == computeRootLeftRightUp(p, left, right, f, seed)
+
+        ensures  computeRootAndLeftSiblingsUp(p, left, right, f, seed).1 
+            == computeLeftSiblingOnNextPathFromLeftRight(p, left, right, f, seed)
+
         decreases p
     {
      if |p| == 1 then
@@ -72,15 +67,15 @@ module IncAlgoV1 {
          *  Otherwise, if p[0] == 1, the sibling for nextPath at this level is a right sibling and
          *  we do not care about the value of the second component, so we copy the previous one in `left`.
          */
-        (r, if first(p) == 0 then valOnPAt else left) 
+        (r, if first(p) == 0 then [seed] else left) 
     else 
         if last(p) == 0 then
             var r := computeRootAndLeftSiblingsUp(
-                    init(p), init(left),  init(right), f, f(seed, last(right)), init(valOnPAt));
-            (r.0, init(left) + [last(valOnPAt)])
+                    init(p), init(left),  init(right), f, f(seed, last(right)));
+            (r.0, init(left) + [seed])
         else      
             var r :=  computeRootAndLeftSiblingsUp(
-                    init(p), init(left), init(right), f, f(last(left), seed), init(valOnPAt));
+                    init(p), init(left), init(right), f, f(last(left), seed));
                 /*  The nextPath is of the form nextPath(init(p)) + [0].
                  *  So the sibling at this level is a right sibling and the value we store in the
                  *  result for this result is irrelevant. We choose to keep the value of the previous left
@@ -90,56 +85,7 @@ module IncAlgoV1 {
     }
 
     //  Correctness proofs.
-
-    /**
-     *  For path of size >= 2, computeRootPathDiffAndLeftSiblingsUp and computeRootLeftRightUp
-     *  yield the same result.
-     *  
-     *  @param  p           The path.
-     *  @param  left        The values of the left siblings of nodes on path `p`.
-     *  @param  right       The values of the left siblings of nodes on path `p`.
-     *  @param  seed        The value at nodeAt(p).
-     *  @param  valOnPAt    The values of the nodes on the path p.
-     *  @param  f           The binary operation to compute.
-     */
-    lemma {:induction p, left, right} computeRootAndSiblingsIsCorrect<T>(p : seq<bit>, left : seq<T>, right: seq<T>, f : (T, T) -> T, seed: T, valOnP: seq<T>) 
-        requires |p| == |left| == |right| == |valOnP|
-        requires |p| >= 1
-        /* We prove the following property: */
-        ensures computeRootAndLeftSiblingsUp(p, left, right, f, seed, valOnP).0 == computeRootLeftRightUp(p, left, right, f, seed)
-        /*  And combining with the post condition of computeRootAndLeftSiblingsUp 
-         *  it gives the following general result: if the returned value is (r, xs)
-         *  1. then r is the same as computeRoot
-         *  2. xs is the the same as the computeLeftSiblingOnNextPath(p)
-         */
-        ensures  computeRootAndLeftSiblingsUp(p, left, right, f, seed, valOnP) == 
-            (computeRootLeftRightUp(p, left, right, f, seed),
-            computeLeftSiblingOnNextPath(p, valOnP, left)
-            )
-        decreases p
-    {
-        if |p| == 1 {
-            //  Thanks Dafny
-            calc == {
-                computeRootAndLeftSiblingsUp(p, left, right, f, seed, valOnP).0;
-                computeRootLeftRightUp(p, left, right, f, seed);
-                { computeLeftRightUpEqualsComputeLeftRight(p, left, right, f, seed); }
-                computeRootLeftRightUp(p, left, right, f, seed);
-            }
-        } else {
-            //  Define result on node according to last(p)
-            var x := if last(p) == 0 then f(seed, last(right)) else  f(last(left), seed);
-            //  Induction on init(p)
-            calc == {
-                    computeRootAndLeftSiblingsUp(p, left, right, f, seed, valOnP).0;
-                    computeRootAndLeftSiblingsUp(init(p), init(left),  init(right), f, x, init(valOnP)).0;
-                    { computeRootAndSiblingsIsCorrect(init(p), init(left), init(right), f,  x, init(valOnP)) ; }
-                    computeRootLeftRightUp(init(p), init(left), init(right), f, x);
-                    computeRootLeftRightUp(p, left, right, f, seed);
-                }
-        }
-    }
-
+   
     /** 
      *  Correctness proof in a tree.
      *  
@@ -147,67 +93,65 @@ module IncAlgoV1 {
      *  @param  r           A complete tree.
      *  @param  left        The values of the left siblings of nodes on path `p` in `r`.
      *  @param  right       The values of the right siblings of nodes on path `p` in `r`.
-     *  @param  valOnPAt    The values of the nodes on the path p.
      *  @param  f           The binary operation to compute.
      *  @param  seed        The value at nodeAt(p) (leaf).
      *  @param  d           The default value for type `T`.
      *  @param  k           The index of a leaf (not last) in `r`.
      */
     lemma {:induction p} computeRootPathDiffAndLeftSiblingsUpInATree<T>(
-            p: seq<bit>, r :  Tree<T>, left: seq<T>, right: seq<T>, valOnP : seq<T>, f : (T, T) -> T, seed : T, d : T, k : nat)
+            p: seq<bit>, r :  Tree<T>, left: seq<T>, right: seq<T>, f : (T, T) -> T, seed : T, d : T, k : nat)
 
         requires isCompleteTree(r)       
         requires isDecoratedWith(f, r)
         requires hasLeavesIndexedFrom(r, 0)
 
-        requires k < |leavesIn(r)|
+        requires k < |leavesIn(r)| - 1
         requires forall i :: k < i < |leavesIn(r)| ==> leavesIn(r)[i].v == d
         requires leavesIn(r)[k].v == seed
 
         /** Path to k-th leaf. */
         requires 1 <= |p| == height(r)   
         requires bitListToNat(p) == k 
-        // nodeAt(p, r) == leavesIn(r)[k]
-        // requires seed == nodeAt(p,r).v 
+
+        requires |left| == |right| == |p|
+
+         /** Left and right contains siblings left and right values.  */
+        requires forall i :: 0 <= i < |p| ==>
+            siblingAt(take(p, i + 1), r).v == 
+                if p[i] == 0 then 
+                    right[i]
+                else 
+                    left[i]
 
         /** Path is not to the last leaf. */
-        requires exists i :: 0 <= i < |p| && p[i] == 0
-        requires |left| == |right| == |valOnP| == |p|
-
-        requires forall i :: 0 <= i < |p| ==> valOnP[i] == nodeAt(take(p, i + 1),r).v 
-
-        /** Left and right contain values of left and siblings of `p` in `r`. */
-        requires forall i :: 0 <= i < |p| ==>
-            (p[i] == 1 && left[i] == siblingAt(take(p, i + 1),r).v)
-            || 
-            (p[i] == 0 && right[i] == siblingAt(take(p, i + 1),r).v)
+        ensures exists i :: 0 <= i < |p| && p[i] == 0
 
         /** Non-optimsied version is correct. */
-        ensures computeRootAndLeftSiblingsUp(p, left, right, f, seed, valOnP).0 == r.v
-        ensures computeRootAndLeftSiblingsUp(p, left, right, f, seed, valOnP).1 
-                                                    == computeLeftSiblingOnNextPath(p, valOnP, left)
+        ensures computeRootAndLeftSiblingsUp(p, left, right, f, seed).0 == r.v
+        ensures forall i :: 0 <= i < |p| && nextPath(p)[i] == 1 ==> 
+                (computeRootAndLeftSiblingsUp(p, left, right, f, seed).1)[i] == siblingAt(take(nextPath(p), i + 1),r).v
 
-        /** Optimsied is correct as they compute the same result. */
-        // ensures computeRootPathDiffAndLeftSiblingsUpOpt(p, v2, seed, v1).0 == r.v
-        // ensures computeRootPathDiffAndLeftSiblingsUpOpt(p, v2, seed, v1).1 
-        //                                             == computeLeftSiblingOnNextPath(p, v1, v2)
     {
-        //  Prove that seed == nodeAt(p, r).v
+        //  exists p[i] == 0, necessary to apply computeLeftSiblingOnNextPathFromLeftRightIsCorrectInATree lemma
+        calc ==> {
+            true;
+            { pathToLeafInInitHasZero(p, r, k); }
+            exists i ::  0 <= i < |p| && p[i] == 0;
+        }
+        
+        //   we have computeRootAndLeftSiblingsUp(p, left, right, f, seed).0 == computeRootLeftRightUp(p, left, right, f, seed)
+        computeLeftRightUpEqualsComputeLeftRight(p, left, right, f, seed);
+
+       //  Prove that seed == nodeAt(p, r).v, ncessary to apply lemma computeRootLeftRightIsCorrectForTree
         calc == {
-            nodeAt(p, r).v;
+            nodeAt(p, r);
             { leafAtPathIsIntValueOfPath(p, r, k, 0) ; }
-            leavesIn(r)[k].v;
-            seed;
+            leavesIn(r)[k];
+            // seed;
         }
-        calc == {
-            computeRootAndLeftSiblingsUp(p, left, right, f, seed, valOnP).0 ;
-            { computeRootAndSiblingsIsCorrect(p, left, right, f, seed, valOnP); }
-            computeRootLeftRightUp(p, left, right, f, seed) ;
-            { computeLeftRightUpEqualsComputeLeftRight(p, left, right, f, seed); }
-            computeRootLeftRight(p, left, right, f, seed) ; 
-            { computeRootLeftRightIsCorrectForTree(p, r, left, right, f, seed) ; }
-            r.v;  
-        }
+        computeRootLeftRightIsCorrectForTree(p, r, left, right, f, seed);
+        
+        computeLeftSiblingOnNextPathFromLeftRightIsCorrectInATree(p, r, left, right, f, seed, k);
     }
 
      /**
@@ -221,43 +165,43 @@ module IncAlgoV1 {
      *  @param  valOnPAt    The values of the nodes on the path p.
      *  @param  f           The binary operation to compute.
      */
-    function computeRootAndLeftSiblingsUpOpt<T>(
-        p : seq<bit>, left : seq<T>, right : seq<T>, f : (T, T) -> T, seed: T, valOnP: seq<T>) : (T, seq<T>)
-        requires |p| == |left| == |right| == |valOnP|
-        requires |p| >= 1
+    // function computeRootAndLeftSiblingsUpOpt<T>(
+    //     p : seq<bit>, left : seq<T>, right : seq<T>, f : (T, T) -> T, seed: T, valOnP: seq<T>) : (T, seq<T>)
+    //     requires |p| == |left| == |right| == |valOnP|
+    //     requires |p| >= 1
 
-        /** Optimised computes same result as non-optimised. */
-        ensures 
-            computeRootAndLeftSiblingsUp(p, left, right, f, seed, valOnP)
-            == 
-            computeRootAndLeftSiblingsUpOpt(p, left, right, f, seed, valOnP)
+    //     /** Optimised computes same result as non-optimised. */
+    //     ensures 
+    //         computeRootAndLeftSiblingsUp(p, left, right, f, seed, valOnP)
+    //         == 
+    //         computeRootAndLeftSiblingsUpOpt(p, left, right, f, seed, valOnP)
 
-        decreases p
-    {
-     if |p| == 1 then
-        var r := computeRootLeftRightUp(p, left, right, f, seed);
-        (r, if first(p) == 0 then valOnP else left) 
-    else 
-        if last(p) == 0 then
-            //  Inline the proof that optimised computes same as non optimised
-            //  Compute resuklt with non-optimised
-            ghost var r1 := computeRootAndLeftSiblingsUp(
-                    init(p), init(left), init(right), f,  f(seed, last(right)), init(valOnP));
+    //     decreases p
+    // {
+    //  if |p| == 1 then
+    //     var r := computeRootLeftRightUp(p, left, right, f, seed);
+    //     (r, if first(p) == 0 then valOnP else left) 
+    // else 
+    //     if last(p) == 0 then
+    //         //  Inline the proof that optimised computes same as non optimised
+    //         //  Compute resuklt with non-optimised
+    //         ghost var r1 := computeRootAndLeftSiblingsUp(
+    //                 init(p), init(left), init(right), f,  f(seed, last(right)), init(valOnP));
             
-            //  This is the optimisation: we compute RootPathDiff only
-            var r := computeRootLeftRightUp(init(p), init(left), init(right), f,  f(seed, last(right)));
-            //  Prove that r1.0 == r
-            calc == {
-                r1.0;
-                {  computeRootAndSiblingsIsCorrect(init(p),  init(left), init(right), f,  f(seed, last(right)),
-                     init(valOnP)) ; }
-                computeRootLeftRightUp(init(p),  init(left), init(right), f,  f(seed, last(right)));
-                r;
-            }
-            (r, init(left) + [last(valOnP)])
-        else      
-            var r :=  computeRootAndLeftSiblingsUpOpt(
-                    init(p), init(left), init(right), f, f(last(left), seed), init(valOnP));
-                    (r.0, r.1 + [last(left)])
-    }
+    //         //  This is the optimisation: we compute RootPathDiff only
+    //         var r := computeRootLeftRightUp(init(p), init(left), init(right), f,  f(seed, last(right)));
+    //         //  Prove that r1.0 == r
+    //         calc == {
+    //             r1.0;
+    //             {  computeRootAndSiblingsIsCorrect(init(p),  init(left), init(right), f,  f(seed, last(right)),
+    //                  init(valOnP)) ; }
+    //             computeRootLeftRightUp(init(p),  init(left), init(right), f,  f(seed, last(right)));
+    //             r;
+    //         }
+    //         (r, init(left) + [last(valOnP)])
+    //     else      
+    //         var r :=  computeRootAndLeftSiblingsUpOpt(
+    //                 init(p), init(left), init(right), f, f(last(left), seed), init(valOnP));
+    //                 (r.0, r.1 + [last(left)])
+    // }
  }
